sources/Facts.v
@@ -1,6 +1,7 @@
-Require Import Main.Stencils Model.
+Require Import Main.Stencils Main.Sets Model.
 
-Require Import Setoid String ZArith.
+Require Import Setoid String ZArith List.
+Import ListNotations.
 Local Open Scope Z_scope.
 
 (* ========================================================================== *)
@@ -90,19 +91,66 @@ Module Make (Cell : CELL) (Stencil : STENCIL Cell).
   End EquivFacts.
 
   (* ======================================================================== *)
+  Module WEquivFacts.
+
+    (** Two states are weakly equivalent if they assign the same value to
+     * variables. *)
+    Definition weak_equiv s t :=
+      forall x, State.get_var s x = State.get_var t x.
+
+    (** If two states are weakly equivalents, updating them (in the same way!)
+     * yields two weakly equivalent states. *)
+    Fact set_var_weq :
+      forall s t,
+        weak_equiv s t -> forall x v, weak_equiv (s⟨x ← v⟩) (t⟨x ← v⟩).
+    Proof.
+      unfold weak_equiv, State.get_var; intros s t H x v x'.
+      destruct s, t; simpl in *.
+      destruct (string_dec x' x); firstorder.
+    Qed.
+
+    (** Arithmetic expressions are invariant through any change of weakly
+     * equivalent state. *)
+    Fact Arith_eval_weq :
+      forall s t,
+        weak_equiv s t -> forall e, Arith.eval s e = Arith.eval t e.
+    Proof.
+      intros s t H; induction e; simpl; try now rewrite IHe1, IHe2.
+      reflexivity.
+      now rewrite H.
+    Qed.
+
+    (** The same results holds for boolean expressions. *)
+    Fact Bool_eval_weq :
+      forall s t,
+        weak_equiv s t -> forall e, Bool.eval s e = Bool.eval t e.
+    Proof.
+      intros s t H; induction e; simpl;
+      try now rewrite (Arith_eval_weq s t H t0), (Arith_eval_weq s t H t1).
+      reflexivity.
+      now rewrite IHe.
+      now rewrite IHe1, IHe2.
+      now rewrite IHe1, IHe2.
+    Qed.
+
+  End WEquivFacts.
+
+  (* ======================================================================== *)
   Module ImpFacts.
 
     (** This module contains results about the simple imperative
      * programs. *)
 
     Import EquivFacts.
+    Import WEquivFacts.
 
     (** Assignments have a limited scope.  Programs are effect-free. *)
     Fact effect_free :
       forall s t p,
-        p // s ⇓ t -> forall x, State.get_var s x = State.get_var t x.
+        p // s ⇓ t -> weak_equiv s t.
     Proof.
-      intros s t p H; induction H; try firstorder.
+      intros s t p H; induction H; try firstorder;
+      unfold weak_equiv in *; intros.
       now rewrite <- IHexec2, <- IHexec1.
       simpl; destruct (string_dec x0 x); subst.
       reflexivity.
@@ -154,30 +202,223 @@ Module Make (Cell : CELL) (Stencil : STENCIL Cell).
   (* ======================================================================== *)
   Module Symbolic.
 
-    Fixpoint eval (p : KStep.t) (s : State.t) : State.t :=
+    (** The correctness of distributed kernels has been defined using traces.
+     * In this module, we take advantage of the fact that Stencil code can be
+     * written using a simple, non Turing-complete language to automatically
+     * synthesize these traces. *)
+
+    Local Open Scope set_scope.
+
+    Definition reflects (s : State.t) (S : set Cell.t) :=
+      forall c, State.get_cell s c = true <-> c ∈ S.
+
+    Fact reflects_same :
+      forall s S1 S2,
+        S1 ≡ S2 -> reflects s S1 -> reflects s S2.
+    Proof. firstorder. Qed.
+
+    Fixpoint exec (p : KStep.t) (s : State.t) : set Cell.t :=
+      match p with
+        | Nop%step_t => ∅
+        | (Fire c)%step_t => ⎨CEval s c⎬
+        | (If b Then p1 Else p2)%step_t =>
+          if Bool.eval s b then exec p1 s else exec p2 s
+        | (p1;; p2)%step_t =>
+          exec p1 s ∪ exec p2 s
+        | (For x From a To b Do q)%step_t =>
+          ⋃⎨exec q (s⟨x ← k⟩), k ∈〚Arith.eval s a , Arith.eval s b〛⎬
+      end.
+
+    Ltac invert_exec :=
+      repeat match goal with
+        | [ H : Imp.exec _ Imp.NoOp _ |- _ ] =>
+          inversion H; clear H; subst
+        | [ H : Imp.exec _ (Imp.Flag _) _ |- _ ] =>
+          inversion H; clear H; subst
+        | [ H : Imp.exec _ (Imp.Cond _ _ _) _ |- _ ] =>
+          inversion H; clear H; subst
+        | [ H : Imp.exec _ (Imp.Seq _ _) _ |- _ ] =>
+          inversion H; clear H; subst
+        | [ H : Imp.exec _ (Imp.Assert _) _ |- _ ] =>
+          inversion H; clear H; subst
+      end.
+
+    Ltac clear_sets :=
+      unfold reflects, same, is_in, bin_union, empty, singleton,
+      seg_union in *.
+
+    Import WEquivFacts.
+
+    (** The symbolic evaluator returns the same set whenever a state [s] is
+     * transformed into another one [t], as long as [t] is weakly equivalent
+     * to [s]. *)
+    Lemma exec_indep :
+      forall p,
+      forall s t,
+        weak_equiv s t -> exec p s ≡ exec p t.
+    Proof.
+      induction p; simpl; intros.
+      + clear_sets; easy.
+      + clear_sets.
+        unfold CEval; intros; split; intros;
+        erewrite Cell.eval_ext; try eassumption.
+        now apply Arith_eval_weq.
+        intros; symmetry; now apply Arith_eval_weq.
+      + erewrite Bool_eval_weq; try eassumption.
+        destruct (Bool.eval t0 t); [now apply IHp1 | now apply IHp2].
+      + admit. (* XXX: FIXME, simple fact from set theory. *)
+      + clear_sets.
+        intro c; split; intro H'.
+        * destruct H' as [k [Hk1 Hk2]].
+          exists k.
+          rewrite (Arith_eval_weq s0 t1 H), (Arith_eval_weq s0 t1 H) in Hk1.
+          intuition.
+          specialize (IHp (s0 ⟨s ← k⟩) (t1 ⟨s ← k⟩)).
+          apply IHp.
+          now apply set_var_weq.
+          assumption.
+        * destruct H' as [k [Hk1 Hk2]].
+          exists k.
+          rewrite (Arith_eval_weq s0 t1 H), (Arith_eval_weq s0 t1 H).
+          intuition.
+          specialize (IHp (s0 ⟨s ← k⟩) (t1 ⟨s ← k⟩)).
+          apply IHp.
+          now apply set_var_weq.
+          assumption.
+    Qed.
+
+    Fact arith_ind :
+      forall P,
+        (forall a b s, Arith.eval s a > Arith.eval s b -> P s a b) ->
+        (forall a b s, Arith.eval s a = Arith.eval s b -> P s a b) ->
+        (forall a b s, Arith.eval s a <= Arith.eval s b -> P s a b ->
+                       P s (1 + a)%arith_t b) ->
+        forall a b s, P s a b.
+    Proof.
+      intros P Hi He Hind a b s.
+      destruct Z_le_gt_dec with (Arith.eval s a) (Arith.eval s b).
+      2: now apply Hi.
+      assert (X : forall k u v, k >= 0 ->
+                                Arith.eval s u + k = Arith.eval s v -> P s u v).
+      induction k.
+      intros; apply He; omega.
+      admit.
+      now destruct 1.
+
+      apply X with (Arith.eval s b - Arith.eval s a); omega.
+    Qed.
+
+    Fact exec_reflects :
+      forall F p s t,
+        (denote p F) // s ⇓ t ->
+        forall S, reflects s S -> reflects t (S ∪ exec p s).
+    Proof.
+      intro F.
+      induction p; simpl; intros.
+      + invert_exec; clear_sets; firstorder.
+      + invert_exec; clear_sets.
+        simpl in *; intros; split; intros;
+        destruct (Cell.eq_dec c0 (CEval t0 c));
+        firstorder.
+      + invert_exec.
+        destruct (Bool.eval s t); [now apply IHp1|now apply IHp2].
+      + invert_exec.
+        apply reflects_same with ((S ∪ exec p1 s) ∪ exec p2 s).
+        admit. (* XXX: FIXME, set theory here *)
+        specialize (IHp1 s t0 H4 S H0).
+        specialize (IHp2 t0 t H6 (S ∪ exec p1 s) IHp1).
+        apply reflects_same with (((S ∪ exec p1 s) ∪ exec p2 t0));
+          [|eassumption].
+        admit. (* XXX: FIXME, set theory again *)
+      + generalize dependent s0; generalize dependent t0; generalize dependent t.
+        apply arith_ind.
+        * intros.
+          inversion H0; clear H0; subst.
+    Abort.
+
+    (*
+    (** Symbolic execution of [KStep.t] programs. *)
+    Fixpoint exec (p : KStep.t) (s : State.t) : State.t :=
       match p with
         | Nop%step_t => s
         | (Fire c)%step_t => State.set_cell s (CEval s c)
         | (If b Then p1 Else p2)%step_t =>
-          if Bool.eval s b then eval p1 s else eval p2 s
+          if Bool.eval s b then exec p1 s else exec p2 s
         | (p1;; p2)%step_t =>
-          eval p2 (eval p1 s)
+          exec p2 (exec p1 s)
         | (For i From a To b Do q)%step_t =>
           s (* XXX: FIXME *)
       end.
 
-    Definition comp_step (k : Kernel.t) (T : Time.t)
+    (** Symbolic execution of computation steps. *)
+    Definition comp_exec (k : Kernel.t) (T : Time.t)
                (s : GState.t) : GState.t :=
-      fun id => eval (Kernel.comp k) ((s id)⟨"id" ← id; "T" ← T⟩).
+      fun id => exec (Kernel.comp k) ((s id)⟨"id" ← id; "T" ← T⟩).
 
-    Definition comm_pat (k : Kernel.t) (T : Time.t) (t : GState.t) :=
+    (** Symbolic execution of communication steps, first part.  Here we
+     * return a description of what each thread sends to each other
+     * thread. *)
+    Definition send_exec (k : Kernel.t) (T : Time.t) :=
       fun id to =>
-        eval (Kernel.comm k) State.initial⟨"id" ← id; "to" ← to; "T" ← T⟩.
+        exec (Kernel.comm k) State.initial⟨"id" ← id; "to" ← to; "T" ← T⟩.
 
-    Definition comm_step (k : Kernel.t) (T : Time.t)
+    (* XXX: This should move. *)
+    Fixpoint ilist' (n : nat) (acc : list Z) : list Z :=
+      match n with
+        | 0%nat => 0 :: acc
+        | S k => ilist' k ((Z.of_nat (S k)) :: acc)
+      end.
+    Definition ilist n := ilist' (Z.to_nat n) nil.
+
+    (** Symbolic execution of communication steps, second part.  It
+     * corresponds to the update of local thread states, after they all
+     * sent what they had to send. *)
+    Definition comm_exec (k : Kernel.t) (T : Time.t) (idMax : Thread.t)
                (t : GState.t) : GState.t :=
-      fun id => State.initial. (* XXX: FIXME *)
+      fun id =>
+        List.fold_right State.union (t id)
+                        (List.map (fun n => send_exec k T n id) (ilist idMax)).
+
+    Module Trace.
+
+      (** [Trace.s], [Trace.t] and [Trace.u] are the synthetic traces, meant to
+       * be used in the kernel correctness statement of the end user's
+       * program. *)
+
+      Definition u (k : Kernel.t) (T : Time.t) (src to : Thread.t) : State.t :=
+        send_exec k T src to.
+
+      Fixpoint st (k : Kernel.t) (T : Time.t) (idMax : Thread.t)
+      : GState.t * GState.t :=
+        match T with
+          | 0%nat => (fun _ => State.initial,
+                      comp_exec k T (fun _ => State.initial))
+          | S T' =>
+            let (_,t) := st k T' idMax in
+            let s := comm_exec k T idMax t in
+            (s, comp_exec k T s)
+        end.
+
+      Definition s k T idMax := fst (st k T idMax).
+      Definition t k T idMax := snd (st k T idMax).
+
+    End Trace.
+*)
   End Symbolic.
+
+  Module SymbFacts.
+(*
+    Theorem trace_gen_correct :
+      forall p Tmax idMax,
+        Kernel.correct p Tmax idMax ->
+        Kernel.trace_correct p Tmax idMax
+                             (fun T => Symbolic.Trace.s p T idMax)
+                             (fun T => Symbolic.Trace.t p T idMax)
+                             (fun T => Symbolic.Trace.u p T).
+    Proof.
+    Abort.
+*)
+  End SymbFacts.
 
   (* ======================================================================== *)
   Module Automation.
@@ -186,7 +427,9 @@ Module Make (Cell : CELL) (Stencil : STENCIL Cell).
 
     (** Syntactic sugar *)
     Tactic Notation "halts" "after" constr(n) "steps" :=
-      exists (n : Z).
+      exists (n : Time.t).
+    Tactic Notation "use" constr(n) "threads" :=
+      exists (n : Thread.t).
 
   End Automation.
 
